theories/program_logic/weakestpre.v
@@ -17,11 +17,11 @@ Definition wp_pre `{irisG Λ Σ} (s : stuckness)
     coPset -c> expr Λ -c> (val Λ -c> iProp Σ) -c> iProp Σ := λ E e1 Φ,
   match to_val e1 with
   | Some v => |={E}=> Φ v
-  | None => ∀ σ1 κs,
-      state_interp σ1 κs ={E,∅}=∗ ⌜if s is NotStuck then reducible e1 σ1 else True⌝ ∗
-      ∀ κ (κs' : list (observation Λ)) e2 σ2 efs, ⌜prim_step e1 σ1 κ e2 σ2 efs ∧ κs = cons_obs κ κs'⌝ ={∅,∅,E}▷=∗
-      state_interp σ2 κs' ∗ wp E e2 Φ ∗
-      [∗ list] ef ∈ efs, wp ⊤ ef (λ _, True)
+  | None => ∀ σ1 κ κs,
+      state_interp σ1 (cons_obs κ κs) ={E,∅}=∗
+        ⌜if s is NotStuck then reducible e1 σ1 else True⌝ ∗
+        ∀ e2 σ2 efs, ⌜prim_step e1 σ1 κ e2 σ2 efs⌝ ={∅,∅,E}▷=∗
+          state_interp σ2 κs ∗ wp E e2 Φ ∗ [∗ list] ef ∈ efs, wp ⊤ ef (λ _, True)
   end%I.
 
 Local Instance wp_pre_contractive `{irisG Λ Σ} s : Contractive (wp_pre s).
@@ -57,7 +57,7 @@ Proof.
   (* FIXME: figure out a way to properly automate this proof *)
   (* FIXME: reflexivity, as being called many times by f_equiv and f_contractive
   is very slow here *)
-  do 24 (f_contractive || f_equiv). apply IH; first lia.
+  do 22 (f_contractive || f_equiv). apply IH; first lia.
   intros v. eapply dist_le; eauto with lia.
 Qed.
 Global Instance wp_proper s E e :
@@ -79,9 +79,9 @@ Proof.
   rewrite !wp_unfold /wp_pre.
   destruct (to_val e) as [v|] eqn:?.
   { iApply ("HΦ" with "[> -]"). by iApply (fupd_mask_mono E1 _). }
-  iIntros (σ1 κs) "Hσ". iMod (fupd_intro_mask' E2 E1) as "Hclose"; first done.
+  iIntros (σ1 κ κs) "Hσ". iMod (fupd_intro_mask' E2 E1) as "Hclose"; first done.
   iMod ("H" with "[$]") as "[% H]".
-  iModIntro. iSplit; [by destruct s1, s2|]. iIntros (κ κs' e2 σ2 efs Hstep).
+  iModIntro. iSplit; [by destruct s1, s2|]. iIntros (e2 σ2 efs Hstep).
   iMod ("H" with "[//]") as "H". iIntros "!> !>". iMod "H" as "($ & H & Hefs)".
   iMod "Hclose" as "_". iModIntro. iSplitR "Hefs".
   - iApply ("IH" with "[//] H HΦ").
@@ -93,7 +93,7 @@ Lemma fupd_wp s E e Φ : (|={E}=> WP e @ s; E {{ Φ }}) ⊢ WP e @ s; E {{ Φ }}
 Proof.
   rewrite wp_unfold /wp_pre. iIntros "H". destruct (to_val e) as [v|] eqn:?.
   { by iMod "H". }
-  iIntros (σ1 κs) "Hσ1". iMod "H". by iApply "H".
+  iIntros (σ1 κ κs) "Hσ1". iMod "H". by iApply "H".
 Qed.
 Lemma wp_fupd s E e Φ : WP e @ s; E {{ v, |={E}=> Φ v }} ⊢ WP e @ s; E {{ Φ }}.
 Proof. iIntros "H". iApply (wp_strong_mono s s E with "H"); auto. Qed.
@@ -104,12 +104,12 @@ Proof.
   iIntros "H". rewrite !wp_unfold /wp_pre.
   destruct (to_val e) as [v|] eqn:He.
   { by iDestruct "H" as ">>> $". }
-  iIntros (σ1 κs) "Hσ". iMod "H". iMod ("H" $! σ1 with "Hσ") as "[$ H]".
-  iModIntro. iIntros (κ κs' e2 σ2 efs [Hstep ->]).
+  iIntros (σ1 κ κs) "Hσ". iMod "H". iMod ("H" $! σ1 with "Hσ") as "[$ H]".
+  iModIntro. iIntros (e2 σ2 efs Hstep).
   iMod ("H" with "[//]") as "H". iIntros "!>!>". iMod "H" as "(Hphy & H & $)". destruct s.
   - rewrite !wp_unfold /wp_pre. destruct (to_val e2) as [v2|] eqn:He2.
     + iDestruct "H" as ">> $". by iFrame.
-    + iMod ("H" with "[$]") as "[H _]". iDestruct "H" as %(? & ? & ? & ? & ?).
+    + iMod ("H" $! _ None with "[$]") as "[H _]". iDestruct "H" as %(? & ? & ? & ? & ?).
       by edestruct (atomic _ _ _ _ _ Hstep).
   - destruct (atomic _ _ _ _ _ Hstep) as [v <-%of_to_val].
     iMod (wp_value_inv' with "H") as ">H". iFrame "Hphy". by iApply wp_value'.
@@ -120,8 +120,8 @@ Lemma wp_step_fupd s E1 E2 e P Φ :
   (|={E1,E2}▷=> P) -∗ WP e @ s; E2 {{ v, P ={E1}=∗ Φ v }} -∗ WP e @ s; E1 {{ Φ }}.
 Proof.
   rewrite !wp_unfold /wp_pre. iIntros (-> ?) "HR H".
-  iIntros (σ1 κs) "Hσ". iMod "HR". iMod ("H" with "[$]") as "[$ H]".
-  iIntros "!>" (κ κs' e2 σ2 efs Hstep). iMod ("H" $! κ κs' e2 σ2 efs with "[% //]") as "H".
+  iIntros (σ1 κ κs) "Hσ". iMod "HR". iMod ("H" with "[$]") as "[$ H]".
+  iIntros "!>" (e2 σ2 efs Hstep). iMod ("H" $! e2 σ2 efs with "[% //]") as "H".
   iIntros "!>!>". iMod "H" as "($ & H & $)".
   iMod "HR". iModIntro. iApply (wp_strong_mono s s E2 with "H"); [done..|].
   iIntros (v) "H". by iApply "H".
@@ -134,12 +134,12 @@ Proof.
   destruct (to_val e) as [v|] eqn:He.
   { apply of_to_val in He as <-. by iApply fupd_wp. }
   rewrite wp_unfold /wp_pre fill_not_val //.
-  iIntros (σ1 κs) "Hσ". iMod ("H" with "[$]") as "[% H]". iModIntro; iSplit.
+  iIntros (σ1 κ κs) "Hσ". iMod ("H" with "[$]") as "[% H]". iModIntro; iSplit.
   { iPureIntro. destruct s; last done.
     unfold reducible in *. naive_solver eauto using fill_step. }
-  iIntros (κ κs' e2 σ2 efs [Hstep ->]).
+  iIntros (e2 σ2 efs Hstep).
   destruct (fill_step_inv e σ1 κ e2 σ2 efs) as (e2'&->&?); auto.
-  iMod ("H" $! κ κs' e2' σ2 efs with "[//]") as "H". iIntros "!>!>".
+  iMod ("H" $! e2' σ2 efs with "[//]") as "H". iIntros "!>!>".
   iMod "H" as "($ & H & $)". by iApply "IH".
 Qed.
 
@@ -150,10 +150,10 @@ Proof.
   destruct (to_val e) as [v|] eqn:He.
   { apply of_to_val in He as <-. by rewrite !wp_unfold /wp_pre. }
   rewrite fill_not_val //.
-  iIntros (σ1 κs) "Hσ". iMod ("H" with "[$]") as "[% H]". iModIntro; iSplit.
+  iIntros (σ1 κ κs) "Hσ". iMod ("H" with "[$]") as "[% H]". iModIntro; iSplit.
   { destruct s; eauto using reducible_fill. }
-  iIntros (κ κs' e2 σ2 efs [Hstep ->]).
-  iMod ("H" $! κ κs' (K e2) σ2 efs with "[]") as "H"; [by eauto using fill_step|].
+  iIntros (e2 σ2 efs Hstep).
+  iMod ("H" $! (K e2) σ2 efs with "[]") as "H"; [by eauto using fill_step|].
   iIntros "!>!>". iMod "H" as "($ & H & $)". by iApply "IH".
 Qed.
 
