theories/program_logic/ectx_lifting.v
@@ -16,28 +16,28 @@ Hint Resolve head_stuck_stuck.
 
 Lemma wp_lift_head_step_fupd {s E Φ} e1 :
   to_val e1 = None →
-  (∀ σ1 κs, state_interp σ1 κs ={E,∅}=∗
+  (∀ σ1 κ κs, state_interp σ1 (cons_obs κ κs) ={E,∅}=∗
     ⌜head_reducible e1 σ1⌝ ∗
-    ∀ κ κs' e2 σ2 efs, ⌜head_step e1 σ1 κ e2 σ2 efs ∧ κs = cons_obs κ κs'⌝ ={∅,∅,E}▷=∗
-      state_interp σ2 κs' ∗ WP e2 @ s; E {{ Φ }} ∗ [∗ list] ef ∈ efs, WP ef @ s; ⊤ {{ _, True }})
+    ∀ e2 σ2 efs, ⌜head_step e1 σ1 κ e2 σ2 efs⌝ ={∅,∅,E}▷=∗
+      state_interp σ2 κs ∗ WP e2 @ s; E {{ Φ }} ∗ [∗ list] ef ∈ efs, WP ef @ s; ⊤ {{ _, True }})
   ⊢ WP e1 @ s; E {{ Φ }}.
 Proof.
-  iIntros (?) "H". iApply wp_lift_step_fupd=>//. iIntros (σ1 κs) "Hσ".
+  iIntros (?) "H". iApply wp_lift_step_fupd=>//. iIntros (σ1 κ κs) "Hσ".
   iMod ("H" with "Hσ") as "[% H]"; iModIntro.
-  iSplit; first by destruct s; eauto. iIntros (κ κs' e2 σ2 efs [Hstep ->]).
+  iSplit; first by destruct s; eauto. iIntros (e2 σ2 efs Hstep).
   iApply "H"; eauto.
 Qed.
 
 Lemma wp_lift_head_step {s E Φ} e1 :
   to_val e1 = None →
-  (∀ σ1 κs, state_interp σ1 κs ={E,∅}=∗
+  (∀ σ1 κ κs, state_interp σ1 (cons_obs κ κs) ={E,∅}=∗
     ⌜head_reducible e1 σ1⌝ ∗
-    ▷ ∀ κ κs' e2 σ2 efs, ⌜head_step e1 σ1 κ e2 σ2 efs ∧ κs = cons_obs κ κs'⌝ ={∅,E}=∗
-      state_interp σ2 κs' ∗ WP e2 @ s; E {{ Φ }} ∗ [∗ list] ef ∈ efs, WP ef @ s; ⊤ {{ _, True }})
+    ▷ ∀ e2 σ2 efs, ⌜head_step e1 σ1 κ e2 σ2 efs⌝ ={∅,E}=∗
+      state_interp σ2 κs ∗ WP e2 @ s; E {{ Φ }} ∗ [∗ list] ef ∈ efs, WP ef @ s; ⊤ {{ _, True }})
   ⊢ WP e1 @ s; E {{ Φ }}.
 Proof.
-  iIntros (?) "H". iApply wp_lift_head_step_fupd; [done|]. iIntros (??) "?".
-  iMod ("H" with "[$]") as "[$ H]". iIntros "!>" (κ κs' e2 σ2 efs ?) "!> !>". by iApply "H".
+  iIntros (?) "H". iApply wp_lift_head_step_fupd; [done|]. iIntros (???) "?".
+  iMod ("H" with "[$]") as "[$ H]". iIntros "!>" (e2 σ2 efs ?) "!> !>". by iApply "H".
 Qed.
 
 Lemma wp_lift_head_stuck E Φ e :
@@ -76,61 +76,61 @@ Qed.
 
 Lemma wp_lift_atomic_head_step_fupd {s E1 E2 Φ} e1 :
   to_val e1 = None →
-  (∀ σ1 κs, state_interp σ1 κs ={E1}=∗
+  (∀ σ1 κ κs, state_interp σ1 (cons_obs κ κs) ={E1}=∗
     ⌜head_reducible e1 σ1⌝ ∗
-    ∀ κ κs' e2 σ2 efs, ⌜head_step e1 σ1 κ e2 σ2 efs ∧ κs = cons_obs κ κs'⌝ ={E1,E2}▷=∗
-      state_interp σ2 κs' ∗
+    ∀ e2 σ2 efs, ⌜head_step e1 σ1 κ e2 σ2 efs⌝ ={E1,E2}▷=∗
+      state_interp σ2 κs ∗
       from_option Φ False (to_val e2) ∗ [∗ list] ef ∈ efs, WP ef @ s; ⊤ {{ _, True }})
   ⊢ WP e1 @ s; E1 {{ Φ }}.
 Proof.
   iIntros (?) "H". iApply wp_lift_atomic_step_fupd; [done|].
-  iIntros (σ1 κs) "Hσ1". iMod ("H" with "Hσ1") as "[% H]"; iModIntro.
-  iSplit; first by destruct s; auto. iIntros (κ κs' e2 σ2 efs [Hstep ->]).
+  iIntros (σ1 κ κs) "Hσ1". iMod ("H" with "Hσ1") as "[% H]"; iModIntro.
+  iSplit; first by destruct s; auto. iIntros (e2 σ2 efs Hstep).
   iApply "H"; eauto.
 Qed.
 
 Lemma wp_lift_atomic_head_step {s E Φ} e1 :
   to_val e1 = None →
-  (∀ σ1 κs, state_interp σ1 κs ={E}=∗
+  (∀ σ1 κ κs, state_interp σ1 (cons_obs κ κs) ={E}=∗
     ⌜head_reducible e1 σ1⌝ ∗
-    ▷ ∀ κ κs' e2 σ2 efs, ⌜head_step e1 σ1 κ e2 σ2 efs ∧ κs = cons_obs κ κs'⌝ ={E}=∗
-      state_interp σ2 κs' ∗
+    ▷ ∀ e2 σ2 efs, ⌜head_step e1 σ1 κ e2 σ2 efs⌝ ={E}=∗
+      state_interp σ2 κs ∗
       from_option Φ False (to_val e2) ∗ [∗ list] ef ∈ efs, WP ef @ s; ⊤ {{ _, True }})
   ⊢ WP e1 @ s; E {{ Φ }}.
 Proof.
   iIntros (?) "H". iApply wp_lift_atomic_step; eauto.
-  iIntros (σ1 κs) "Hσ1". iMod ("H" with "Hσ1") as "[% H]"; iModIntro.
-  iSplit; first by destruct s; auto. iNext. iIntros (κ κs' e2 σ2 efs [Hstep ->]).
+  iIntros (σ1 κ κs) "Hσ1". iMod ("H" with "Hσ1") as "[% H]"; iModIntro.
+  iSplit; first by destruct s; auto. iNext. iIntros (e2 σ2 efs Hstep).
   iApply "H"; eauto.
 Qed.
 
-Lemma wp_lift_atomic_head_step_no_fork_fupd {s E1 E2 Φ} e1 :
+Lemma wp_lift_atomic__head_step_no_fork_fupd {s E1 E2 Φ} e1 :
   to_val e1 = None →
-  (∀ σ1 κs, state_interp σ1 κs ={E1}=∗
+  (∀ σ1 κ κs, state_interp σ1 (cons_obs κ κs) ={E1}=∗
     ⌜head_reducible e1 σ1⌝ ∗
-    ∀ κ κs' e2 σ2 efs, ⌜head_step e1 σ1 κ e2 σ2 efs ∧ κs = cons_obs κ κs'⌝ ={E1,E2}▷=∗
-      ⌜efs = []⌝ ∗ state_interp σ2 κs' ∗ from_option Φ False (to_val e2))
+    ∀ e2 σ2 efs, ⌜head_step e1 σ1 κ e2 σ2 efs⌝ ={E1,E2}▷=∗
+      ⌜efs = []⌝ ∗ state_interp σ2 κs ∗ from_option Φ False (to_val e2))
   ⊢ WP e1 @ s; E1 {{ Φ }}.
 Proof.
   iIntros (?) "H". iApply wp_lift_atomic_head_step_fupd; [done|].
-  iIntros (σ1 κs) "Hσ1". iMod ("H" $! σ1 κs with "Hσ1") as "[$ H]"; iModIntro.
-  iIntros (κ κs' v2 σ2 efs [Hstep ->]).
-  iMod ("H" $! κ κs' v2 σ2 efs with "[# //]") as "H".
+  iIntros (σ1 κ κs) "Hσ1". iMod ("H" $! σ1 with "Hσ1") as "[$ H]"; iModIntro.
+  iIntros (v2 σ2 efs Hstep).
+  iMod ("H" $! v2 σ2 efs with "[# //]") as "H".
   iIntros "!> !>". iMod "H" as "(% & $ & $)"; subst; auto.
 Qed.
 
 Lemma wp_lift_atomic_head_step_no_fork {s E Φ} e1 :
   to_val e1 = None →
-  (∀ σ1 κs, state_interp σ1 κs ={E}=∗
+  (∀ σ1 κ κs, state_interp σ1 (cons_obs κ κs) ={E}=∗
     ⌜head_reducible e1 σ1⌝ ∗
-    ▷ ∀ κ κs' e2 σ2 efs, ⌜head_step e1 σ1 κ e2 σ2 efs ∧ κs = cons_obs κ κs'⌝ ={E}=∗
-      ⌜efs = []⌝ ∗ state_interp σ2 κs' ∗ from_option Φ False (to_val e2))
+    ▷ ∀ e2 σ2 efs, ⌜head_step e1 σ1 κ e2 σ2 efs⌝ ={E}=∗
+      ⌜efs = []⌝ ∗ state_interp σ2 κs ∗ from_option Φ False (to_val e2))
   ⊢ WP e1 @ s; E {{ Φ }}.
 Proof.
   iIntros (?) "H". iApply wp_lift_atomic_head_step; eauto.
-  iIntros (σ1 κs) "Hσ1". iMod ("H" $! σ1 with "Hσ1") as "[$ H]"; iModIntro.
-  iNext; iIntros (κ κs' v2 σ2 efs Hstep).
-  iMod ("H" $! κ κs' v2 σ2 efs with "[# //]") as "(% & $ & $)". subst; auto.
+  iIntros (σ1 κ κs) "Hσ1". iMod ("H" $! σ1 with "Hσ1") as "[$ H]"; iModIntro.
+  iNext; iIntros (v2 σ2 efs Hstep).
+  iMod ("H" $! v2 σ2 efs with "[# //]") as "(% & $ & $)". subst; auto.
 Qed.
 
 Lemma wp_lift_pure_det_head_step {s E E' Φ} e1 e2 efs :
